\chapterimage{chapter_head_2.pdf}
\chapter{Number}

\begin{bxTip}{Skill: BEDMAS}
    \tcblower
    \begin{enumerate}[leftmargin=0cm] 
        \item If $a=2$ and $b=5$, find the value of each expression.

        \begin{tasks}[label=(\alph*), after-item-skip=2pt,after-skip=3pt, label-width=4ex](2)
            \task  $ 3a+4b=$                           \begin{envFillIn}$  -2     $    \end{envFillIn}
            \task  $ \frac{10a}{b}=$                   \begin{envFillIn}$   5     $    \end{envFillIn}
            \task  $ 4a(b-a)=$                         \begin{envFillIn}$  -8     $    \end{envFillIn}
        \end{tasks}
    \end{enumerate}

\end{bxTip}






\begin{bxExample}{Example}    
    \textbf{Example} \begin{itemize} 
	\item[]	Work out $103\frac{7}{8}+4\frac{5}{6} $

	\end{itemize}
\tcbline 

Solution:
\vspace{0.5cm} 

    $\begin{WithArrows}[tikz=blue]
       \qquad    &   103\frac{7}{8}+4\frac{5}{6}  	                 \Arrow{Change to same denonminator}\\[10pt]
	             & =  103\frac{21}{24}+4\frac{20}{24}                     \Arrow{Fraction Addition}     \\[10pt]
                 & = 107\frac{21+20}{24}                                                                \\
                 & = 108\frac{17}{24}			 
    \end{WithArrows}$

\end{bxExample}


\begin{bxExample}{Example}    
    \textbf{Example} Work out $ 28\frac{3}{4}-12\frac{5}{6} $
\tcbline 

Solution:\indent \indent \indent \indent
\vspace{0.5cm} 

    $\begin{WithArrows}[tikz=blue]
       \qquad    &    28\frac{9}{12}-12\frac{10}{12}  	                 \Arrow{Change to same denonminator}               \\[10pt]
	             & =  27\frac{25}{12}-12\frac{27}{12}                     \Arrow{Compare $\frac{25}{30} \;\; \frac{27}{30} $}     \\[10pt]
                 & =  15\frac{25+3}{30}                                                                    \\
                 & =  15\frac{28}{30}			                                                        
    \end{WithArrows}$

\end{bxExample}

\clearpage    



\clearpage    
\begin{enumerate} [leftmargin=0cm]



\item Work out
\begin{tasks}[label=(\alph*), after-item-skip=2pt,after-skip=3pt, label-width=4ex](2)
    \task  $ -5+3=$                           \begin{envFillIn}$  -2     $    \end{envFillIn}
    \task  $ -5+10=$                          \begin{envFillIn}$   5     $    \end{envFillIn}
    \task  $ -5-3=$                           \begin{envFillIn}$  -8     $    \end{envFillIn}
    \task  $ -5+1=$                           \begin{envFillIn}$  -4     $    \end{envFillIn}
    \task  $ -5-(-10)=$                       \begin{envFillIn}$   5     $    \end{envFillIn}
    \task  $ 10-(-10)=$                       \begin{envFillIn}$  20     $    \end{envFillIn}
    \task  $ 10+(-20)=$                       \begin{envFillIn}$ -10     $    \end{envFillIn}
    \task  $ 310+(-420)=$                     \begin{envFillIn}$ -110    $    \end{envFillIn}
    \task  $ -310+(-420)=$                    \begin{envFillIn}$ -730    $    \end{envFillIn}
    \task  $ (-310)+(-420)=$                  \begin{envFillIn}$ -730    $    \end{envFillIn}
    \task  $ (-30)+(-20)+(-10)=$              \begin{envFillIn}$ -60     $    \end{envFillIn}    
    \task  $ -50-30-20=$                      \begin{envFillIn}$ -100    $    \end{envFillIn}    
\end{tasks}


\item   Find the value of              
 \begin{tasks}[label=(\alph*), after-item-skip=2pt,after-skip=3pt, label-width=4ex](2)               
  \task $-10+27 =$        \begin{envFillIn}$     -8  $ \end{envFillIn}
  \task $ -5+3 = $        \begin{envFillIn}$     -2  $ \end{envFillIn}
  \task $ -5-1 =$        \begin{envFillIn}$     -6  $ \end{envFillIn}
  \task $ -15-1 = $        \begin{envFillIn}$     -16  $ \end{envFillIn}
  \task $ -35-1 = $        \begin{envFillIn}$     -36  $ \end{envFillIn}
  \task $ -5-31 = $        \begin{envFillIn}$     -36  $ \end{envFillIn}
 \end{tasks}               


\item Find the value of
\begin{tasks}[label=(\alph*), after-item-skip=2pt,after-skip=3pt, label-width=4ex](2)
    \task  $ -5 \times -2 =                 $                           \begin{envFillIn}$  10      $ \end{envFillIn}
    \task  $ -5 \times (-2) =               $                           \begin{envFillIn}$  10      $    \end{envFillIn}
    \task  $  6 \times -7 =                 $                           \begin{envFillIn}$  -42     $    \end{envFillIn}
    \task  $ -5 \times 9 =                  $                           \begin{envFillIn}$  -45     $    \end{envFillIn}
    \task  $ -8 \times -9 \times -1 =       $                           \begin{envFillIn}$  72      $    \end{envFillIn}
    \task  $ -3 \times 29 =                 $                           \begin{envFillIn}$  -87     $    \end{envFillIn}
\end{tasks}

\item Find the value of
\begin{tasks}[label=(\alph*), after-item-skip=2pt,after-skip=3pt, label-width=4ex](2)
    \task  $ -57 \div  (-3) =               $                           \begin{envFillIn}$  19      $    \end{envFillIn}
    \task  $ 12 \div  -3 =                  $                           \begin{envFillIn}$  -4      $    \end{envFillIn}
    \task  $ -81 \div  3 =                  $                           \begin{envFillIn}$  -27     $    \end{envFillIn}
    \task  $ 12 \div (-4) \times (-3)=      $                           \begin{envFillIn}$  9       $    \end{envFillIn}
\end{tasks}

\item Find the value of
\begin{tasks}[label=(\alph*), after-item-skip=2pt,after-skip=3pt, label-width=4ex](2)
    \task  $ \frac{24}{-3}=              $                              \begin{envFillIn}$  -8                $    \end{envFillIn}
    \task  $ \frac{-24}{-6}=             $                              \begin{envFillIn}$  4                 $    \end{envFillIn}
    \task  $ \frac{-72}{-24}=            $                              \begin{envFillIn}$  3                 $    \end{envFillIn}
    \task  $ \frac{-24}{-6}=             $                              \begin{envFillIn}$  4                 $    \end{envFillIn}
    \task  $ \frac{19}{-57}=             $                              \begin{envFillIn}$  -\frac{1}{3}      $    \end{envFillIn}
    \task  $ \frac{-4}{-16}=             $                              \begin{envFillIn}$  \frac{1}{4}       $    \end{envFillIn}
    \task  $ \frac{-4+6}{-16+8}=         $                              \begin{envFillIn}$  -\frac{1}{4}      $    \end{envFillIn}
\end{tasks}

\item Work out
\begin{tasks}[label=(\alph*), after-item-skip=2pt,after-skip=3pt, label-width=4ex](2)
    \task  $ 10 -  2 \times 5                                    $                 \\  \begin{envAnswer}[blankline=3]        $    0    $ \end{envAnswer}
    \task  $ 10 +  2 \times 5                                    $                 \\  \begin{envAnswer}[blankline=3]        $   20    $ \end{envAnswer}
    \task  $ 10 - 2 +4                                           $                 \\  \begin{envAnswer}[blankline=3]        $   12    $ \end{envAnswer}
    \task  $ 10 - 4 + 2                                          $                 \\  \begin{envAnswer}[blankline=3]        $    8    $ \end{envAnswer}
    \task  $ 10 - (4 + 2)                                        $                 \\  \begin{envAnswer}[blankline=3]        $    4    $ \end{envAnswer}
    \task  $ 60 \div 6 \times 10                                 $                 \\  \begin{envAnswer}[blankline=3]        $  100    $ \end{envAnswer}
    \task  $ 60 -  2 \times 10                                   $                 \\  \begin{envAnswer}[blankline=3]        $   40    $ \end{envAnswer}
    \task  $ 60 -  12 \div  (2 +1) \times 2                      $                 \\  \begin{envAnswer}[blankline=5]        $   52    $ \end{envAnswer}    
    \task  $ 4 \times 5 -  6^2 \div  (2 +1) \times 2 \times 3    $                 \\  \begin{envAnswer}[blankline=5]        $  -52    $ \end{envAnswer}    
\end{tasks}

\item Work out
\begin{tasks}[label=(\alph*), after-item-skip=2pt,after-skip=3pt, label-width=4ex](2)
    \task  $ \frac{8+4}{8 \times 4}                              $                  \\  \begin{envAnswer}[blankline=3]        $       $ \end{envAnswer}
    \task  $ \frac{10+5 \times 2}{5 \div 3} - 1 \frac{1}{4}      $                  \\  \begin{envAnswer}[blankline=3]        $       $ \end{envAnswer}
\end{tasks}

\item Work out
\begin{tasks}[label=(\alph*), after-item-skip=2pt,after-skip=3pt, label-width=4ex](2)
    \task  $ -5^2                                                $                  \\  \begin{envAnswer}[blankline=2]        $       $ \end{envAnswer}
    \task  $ (-5)^2                                              $                  \\  \begin{envAnswer}[blankline=2]        $       $ \end{envAnswer}
    \task  $ (-1)^{200}                                          $                  \\  \begin{envAnswer}[blankline=2]        $       $ \end{envAnswer}
    \task  $ (-1)^{201}                                          $                  \\  \begin{envAnswer}[blankline=2]        $       $ \end{envAnswer}
    \task  $ 12^2                                                $                  \\  \begin{envAnswer}[blankline=2]        $       $ \end{envAnswer}
    \task  $ 19^2                                                $                  \\  \begin{envAnswer}[blankline=2]        $       $ \end{envAnswer}
    \task  $ \sqrt{16+9}                                         $                  \\  \begin{envAnswer}[blankline=2]        $       $ \end{envAnswer}
    \task  $ \sqrt{3^2 + 4^2}                                    $                  \\  \begin{envAnswer}[blankline=2]        $       $ \end{envAnswer}
\end{tasks}


\item Calculate the following. You must show your working.
\begin{tasks}[label=(\alph*), after-item-skip=2pt,after-skip=3pt, label-width=4ex](2)
    \task  $ 3 \times (8-3) - (4-7) \times 5               $                  \\  \begin{envAnswer}[blankline=5]        $       $ \end{envAnswer}
    \task  $ 2^{10}-(-2)^{10} \times 1 \frac{1}{8}               $                  \\  \begin{envAnswer}[blankline=5]        $       $ \end{envAnswer}
    \task  $ 1-(-2)^{10} \times 1 \frac{1}{8}                  $                  \\  \begin{envAnswer}[blankline=5]        $       $ \end{envAnswer}
    \task  $ \sqrt{3^2 + 4^2}                              $                  \\  \begin{envAnswer}[blankline=5]        $       $ \end{envAnswer}
\end{tasks}


\item   How many zeros at the end of $2^{125} \times 5^{200}$? Show your working clearly.       \begin{envAnswer}[blankline= 2 ] $  $ \end{envAnswer}

\item   How many zeros at the end of $7\times 119 \times 2^{125} \times 5^{200}$? Show your working clearly.        \begin{envAnswer}[blankline= 2 ] $  $ \end{envAnswer}

\item   How many zeros at the end of $4^{15} \times 5^{25}$? Show your working clearly.       \begin{envAnswer}[blankline= 2 ] $  $ \end{envAnswer}

\item   How many zeros at the end of $4^{15} \times 5^{25}$? Show your working clearly.        \begin{envAnswer}[blankline= 2 ] $  $ \end{envAnswer}

\item   How many zeros at the end of $32 \times 2^3 \times 125^2$? Show your working clearly.       \begin{envAnswer}[blankline= 2 ] $  $ \end{envAnswer}
                
                
\item   The $n$th term of a squence is $6n+5$. \\            
   Write down the first three terms of this sequence. \\      \begin{envAnswer}[blankline= 2 ] $  $ \end{envAnswer}
                
\item   The $n$th term of a squence is $6n-5$. \\            
   Write down the first three terms of this sequence. \\      \begin{envAnswer}[blankline= 2 ] $  $ \end{envAnswer}

\item   The $n$th term of a squence is $21-4n$. \\             
   Write down the first three terms of this sequence. \\       \begin{envAnswer}[blankline= 2 ] $  $ \end{envAnswer}

\item   The $n$th term of a squence is $n^2-n+1$. \\             
   Write down the first three terms of this sequence. \\       \begin{envAnswer}[blankline= 2 ] $  $ \end{envAnswer}

\item   The $n$th term of a squence is $4n^2+4n+1$. \\             
   Write down the first three terms of this sequence. \\       \begin{envAnswer}[blankline= 2 ] $  $ \end{envAnswer}















\end{enumerate}

\clearpage
