\clearpage
\begin{enumerate} [leftmargin=0cm] 

\item Simplify the following expressions by adding or subtracting like terms.
\begin{tasks}[label=(\alph*), after-item-skip=2pt,after-skip=3pt, label-width=4ex](2)
    \task  $ 3x+5x=           $                               \begin{envFillIn} $  8x         $ \end{envFillIn}
    \task  $ 10x-7x=          $                               \begin{envFillIn} $  3x         $ \end{envFillIn}
    \task  $ -3x+5x=          $                               \begin{envFillIn} $  2x         $ \end{envFillIn}
    \task  $ -10x-7x=         $                               \begin{envFillIn} $  -17x       $ \end{envFillIn} 
\end{tasks}

\item Simplify the following expressions by adding or subtracting like terms.
\begin{tasks}[label=(\alph*), after-item-skip=2pt,after-skip=3pt, label-width=4ex](2)
    \task  $ 3x^2+5x^2=           $                               \begin{envFillIn} $  8x^2         $ \end{envFillIn}
    \task  $ 10^2-7x^2=           $                               \begin{envFillIn} $  3x^2         $ \end{envFillIn}
    \task  $ -3x^2+5x^2=          $                               \begin{envFillIn} $  2x^2         $ \end{envFillIn}
    \task  $ -10x^2-7x^2=         $                               \begin{envFillIn} $  -17x^2       $ \end{envFillIn} 
\end{tasks}

\item Simplify the following expressions by adding or subtracting like terms.
\begin{tasks}[label=(\alph*), after-item-skip=2pt,after-skip=3pt, label-width=4ex](2)
    \task  $ 3x^2+5x+6x^2=           $                               \begin{envFillIn} $  9x^2 +5x        $ \end{envFillIn}
    \task  $ 10x^2+20x^2-7x=         $                               \begin{envFillIn} $  30x^2-7x        $ \end{envFillIn}
    \task  $ 6x^2-3x-7x^2=           $                               \begin{envFillIn} $  -x^2-3x         $ \end{envFillIn}
    \task  $ 5a^2+6a^2-3a=           $                               \begin{envFillIn} $  11a^2-3a        $ \end{envFillIn} 
\end{tasks}


\item Simplify the following expressions by adding or subtracting like terms.
\begin{tasks}[label=(\alph*), after-item-skip=2pt,after-skip=3pt, label-width=4ex](2)
    \task  $ 3x^3+5x^3=           $                               \begin{envFillIn} $  8x^3         $ \end{envFillIn}
    \task  $ 10x^3-7x^3=          $                               \begin{envFillIn} $  3x^3         $ \end{envFillIn}
    \task  $ -3x^3+5x^3=          $                               \begin{envFillIn} $  2x^3         $ \end{envFillIn}
    \task  $ -10x^3-7x^3=         $                               \begin{envFillIn} $  -17x^3       $ \end{envFillIn} 
\end{tasks}

	
\item Simplify the following expressions by adding or subtracting like terms.
\begin{tasks}[label=(\alph*), after-item-skip=2pt,after-skip=3pt, label-width=4ex](2)
    \task  $ 10a-3b+5a-6b=    $                              \begin{envFillIn} $  15a-9b         $ \end{envFillIn}
    \task  $ 10a-3b+5a+6b=    $                              \begin{envFillIn} $  15a+3b         $ \end{envFillIn}
    \task  $ 10a-3b-5a-6b=    $                              \begin{envFillIn} $  5a-9b          $ \end{envFillIn}
    \task  $ 7m-5n+4m-2n=     $                              \begin{envFillIn} $  11m-7n         $ \end{envFillIn}
    \task  $ 7m-5n-4m-2n=     $                              \begin{envFillIn} $  3m-7n          $ \end{envFillIn}
    \task  $ 7m+5n-4m-2n=     $                              \begin{envFillIn} $  3m+3n          $ \end{envFillIn}
    \task  $ 7m+5n-4m+2n=     $                              \begin{envFillIn} $  3m+7n          $ \end{envFillIn}
  
\end{tasks}


\item Simplify.
\begin{tasks}[label=(\alph*), after-item-skip=2pt,after-skip=3pt, label-width=4ex](2)
    \task  $ 5x  \times 4x =                                  $            \begin{envFillIn} $  20x^2         $ \end{envFillIn}
    \task  $ x^4 \times x^2=                                  $            \begin{envFillIn} $  x^6           $ \end{envFillIn}
    \task  $ 5x^2 \times 2x^2=                                $            \begin{envFillIn} $  10x^4         $ \end{envFillIn}
  
\end{tasks}


\item Simplify.
\begin{tasks}[label=(\alph*), after-item-skip=2pt,after-skip=3pt, label-width=4ex](2)
    \task  $ \frac{2}{6x}=                                     $            \begin{envFillIn} $  \frac{1}{3x}        $ \end{envFillIn}
    \task  $ \frac{t^9}{t^3}=                                  $            \begin{envFillIn} $  t^6                 $ \end{envFillIn}
    \task  $ \frac{x^8}{x^2}=                                  $            \begin{envFillIn} $  x^2                 $ \end{envFillIn}
    \task  $ \frac{a^{10}}{a^2}=                               $            \begin{envFillIn} $  a^8                 $ \end{envFillIn}
    \task  $ \frac{a^{12}}{a^2}=                               $            \begin{envFillIn} $  a^{10}              $ \end{envFillIn}
    \task  $ \frac{t^9}{t^3}=                                  $            \begin{envFillIn} $  t^6                 $ \end{envFillIn}
    \task  $ \frac{8x^8}{2x^2}=                                $            \begin{envFillIn} $  4x^2                $ \end{envFillIn}
    \task  $ \frac{x^2}{x^8}=                                  $            \begin{envFillIn} $  \frac{1}{x^6}       $ \end{envFillIn}
  
\end{tasks}


% \item If $m=2x^3-4x^2-7$ and $n=-4x^3-4x^2+5x+8$, what is $m-n$ in terms of $x$? 
% \begin{tasks}[label=\Alph*), after-item-skip=2pt,after-skip=3pt, label-width=4ex](4)
    % \task  $ 6x^3+5x-15                                        $        
    % \task  $ 6x^3-8x^2-5x-15                                   $     
    % \task  \MyCorrectSmartChoice[thick,rounded corners,red]{The writter of this post}	
    % \task  $ -2x^3-8x^2 +5x+1                          ã€€      $             
    % \task  $ 6x^3 -5x-15                                       $             
  
% \end{tasks}


\end{enumerate}